We now implement mutable objects. We start with inheritance:
\begin{lstlisting}
instance (Recursive o, Record o St) => Object o St where
  data Method St ro a b = StMethod(ro -> a -> (b,ro))
  self_ref <=| (StLabel read write) = 
             \x -> do self <- eval self_ref
                      let (StMethod m) = read self
                          (res,self' :: Rec o) = m (to self) x
                      self_ref .= (from self')
                      return res
  mk_method m = StMethod(\this -> \args -> let (St res_st) = m id_ref args
                                               (res,this' :: o) = res_st ((from this) :: o)
                                           in (res,((to this') :: Rec o)))
                where id_ref = StRef (St (\s -> (s,s))) (\s' -> (St (\s -> ((),s'))))
\end{lstlisting}
In our mutable encoding the first field of the object must be either the value of the inherited value or unit when the object does not inherit anything.

Methods enjoy the same implementation in both cases, so we just give one:
\begin{lstlisting}
instance (Object o St, o ~ (Malloc (Inherit b) so)) => Inherits o b St where
  data Inherit a = StInherit a
  get_base self_ref =   StRef(do ((StInherit base) `Malloc` tl) <- eval self_ref
                                 return base)
                             (\base' -> do (_ `Malloc` tl) <- eval self_ref
                                           self_ref .= ((StInherit base') `Malloc` tl)
                                           return ())
\end{lstlisting}

It can prove very useful to take advantage of our existing infrastructure to create methods from references and statements, so that the user of our system will not be forced to define methods by explicitly tracking mutations to the value of $this$; for this reason we add a function to the $Object$ predicate that converts a method from reference to state into our format (the implementation here is the same for both instances of $Object$, so we provide only one:
\begin{lstlisting}
instance (Inherits o b st, Memory s) => Coercible (Ref st s o) (Ref st s b) where
  coerce = get_base
         in res_st this)
\end{lstlisting}